% === Exercise 9.14 ===
\begin{Exercise}
	\begin{enumerate}[(a)]
		\item 		
		\begin{proof}
			For $(x,y) = (0,0)$, we observe
			\begin{align*}
			D_1 f(0,0) 
			&= \lim_{h\to 0} \frac{f(h,0)-f(0,0)}{h-0} 
			= \frac{h-0}{h} 
			= 1; \\
			D_2 f(0,0) 
			&= \lim_{k\to 0} \frac{f(0,k)-f(0,0)}{k-0} 
			= \frac{0-0}{k} 
			= 0.
			\end{align*}
			Notice that $|2xy| \leq x^2+y^2$.
			For $(x,y) \neq (0,0)$, we have
			\begin{align*}
			|D_1 f(x,y)|
			&= \left| \frac{x^4+3x^2 y^2}{(x^2+y^2)^2} \right|
			\leq \frac{3(x^4+x^2 y^2)}{(x^2+y^2)^2}
			= \frac{3x^2}{x^2+y^2}
			\leq 3; \\
			|D_2 f(x,y)|
			&= \left| \frac{2x^3 y}{(x^2+y^2)^2} \right|
			\leq \frac{x^2(x^2+y^2)}{(x^2+y^2)^2}
			= \frac{x^2}{x^2+y^2}
			\leq 1.
			\end{align*}
			Hence $D_1 f$ and $D_2 f$ are bounded functions on $\mathbb{R}^2$.
		\end{proof}
		
		\item
		\begin{proof}
			Put $u = (\cos \theta, \sin \theta)$.
			Consider
			$$
			|D_u f(0,0)|
			= \left| \lim_{h\to 0}\frac{f(hu) - f(0,0)}{\|hu - (0,0) \|}\right|
			= \left| \lim_{h\to 0} \frac{h\cos^3 \theta - 0}{h} \right|
			= |\cos^3 \theta|.
			$$
			Since $|\cos\theta|\leq 1$ and then $|\cos^3 \theta| \leq 1$ follows, we conclude $|D_u f(0,0)|\leq 1$.
		\end{proof}
		
		\item
		\begin{proof}
			(Omitted)
		\end{proof}
		
		\item
		\begin{proof}
			Put $u = \left(\frac{\sqrt{2}}{2}, \frac{\sqrt{2}}{2}\right)$.
			Consider
			$$
			D_u f(0,0) = \left(\frac{\sqrt{2}}{2}\right)^3
			= \frac{\sqrt{2}}{4}.
			$$
			On the other hand,
			$$
			D_1 f(0,0) u_1 + D_2 f(0,0) u_2
			= \frac{\sqrt{2}}{2}\cdot 1 + \frac{\sqrt{2}}{2}\cdot 0
			= \frac{\sqrt{2}}{2}.
			$$
			These mean $D_u f(0,0) \neq D_1 f(0,0) u_1 + D_2 f(0,0) u_2$.
			That is, formula (40) fails.
			
			We conclude $f$ is not differentiable at $(0,0)$.
		\end{proof}
	\end{enumerate}
\end{Exercise}