% === Exercise 3.5 ===
\begin{Exercise}
	\begin{proof}
		Let $a^*=\limsup_{n\to\infty} a_n$, $b^*=\limsup_{n\to\infty} b_n$ and $s^*=\limsup_{n\to\infty} (a_n + b_n)$.
		
		\begin{itemize}
			\item \textbf{$a^*$ and $b^*$ are finite.}
			
			By theorem 3.17(a), we know there exists subsequences $\{a_{n_k}\}, \{b_{n_k}\}$ such that
			$$
			\lim_{k\to\infty} (a_{n_k} + b_{n_k})
			= \lim_{k\to\infty} a_{n_k} + \lim_{k\to\infty} b_{n_k}
			= s^*.
			$$
			Since $\lim_{k\to\infty} a_{n_k} \leq a^*$ and $\lim_{k\to\infty} b_{n_k} \leq b^*$, then $s^* \leq a^* + b^*$.
			It follows that
			$$
			\limsup_{n\to\infty} (a_n + b_n)
			\leq \limsup_{n\to\infty} a_n + \limsup_{n\to\infty} b_n
			$$.
			
			\item \textbf{$a^*=\infty$ and $b^*=\infty$.}
			
			$\infty \leq \infty + \infty$ holds trivially.
			
			\item \textbf{$a^*=-\infty$ and $b^*=-\infty$.}
			
			$-\infty \leq -\infty + -\infty$ holds trivially.
		\end{itemize}
	\end{proof}
\end{Exercise}