% === Exercise 3.4 ===
\begin{Exercise}
	\begin{proof}
		From definition, we know $s_1 = s_2 = 0$ and $s_{2m+2} = \frac{s_{2m+1}}{2} = \frac{1}{4} + \frac{1}{2}s_{2m}$. Then,
		$$
		\lim_{m\to\infty} s_{2m}
		= \frac{1}{4} + \frac{1}{8} + \cdots
		= \sum_{n=1}^{\infty} \frac{1}{2^{n+1}}
		= \frac{\frac{1}{4}}{1 - \frac{1}{2}}
		= \frac{1}{2}.
		$$
		And,
		$$
		\lim_{m\to\infty} s_{2m+1} 
		= \frac{1}{2} + \frac{1}{4} + \cdots
		= \sum_{n=1}^{\infty} \frac{1}{2^n}
		= \frac{\frac{1}{2}}{1 - \frac{1}{2}}
		= 1.
		$$
		As $n$ increase, $s_n$ is close to either $\frac{1}{2}$ or $1$.
		
		We conclude $\liminf_{n\to\infty} s_n = \frac{1}{2}$ and $\limsup_{n\to\infty} s_n = 1$.
	\end{proof}
\end{Exercise}