% === Exercise 3.6 ===
\begin{Exercise}
	\begin{enumerate}[a)]
		\item
		\begin{answer}
			$\sum a_n$ diverges.
		\end{answer}
		\begin{solution}
			We know
			$$
			\sum_{n=1}^{m} a_n
			= (\sqrt{2} - 1) + (\sqrt{3} - \sqrt{2}) + \cdots + (\sqrt{m+1} - \sqrt{m})
			= \sqrt{m+1} - 1.
			$$
			Hence
			$$
			\sum_{n=1}^{\infty} a_n
			= \lim_{m\to\infty} \sum_{n=1}^{m} a_n
			= \infty.
			$$
		\end{solution}
	
		\item
		\begin{answer}
			$\sum a_n$ converges.
		\end{answer}
		\begin{solution}
			We know
			$$
			a_n
			= \frac{\sqrt{n+1} - \sqrt{n}}{n}
			= \frac{\sqrt{n+1} - \sqrt{n}}{n} \cdot \frac{\sqrt{n+1}+\sqrt{n}}{\sqrt{n+1}+\sqrt{n}}
			= \frac{1}{\sqrt{n^3+n^2} + \sqrt{n^3}}
			\leq \frac{1}{2} \cdot \frac{1}{n^{\frac{3}{2}}}.
			$$
			By the p-Series Test (Theorem 3.28), we derive $\sum_{n=1}^{\infty} \sqrt{1}{n^{\frac{3}{2}}}$ converges.
			Moreover, by the Comparison Test (Theorem 3.25), we conclude $\sum a_n$ converges.
		\end{solution}
	\end{enumerate}
\end{Exercise}