% === Exercise 6.11 ===
\begin{Exercise}
	\begin{proof}
		Notice that by Exercise 6.10(c), we have
		\begin{align*}
		\int_{a}^{b}|f-g| |g-h|\,d\alpha
		&= \left| \int_{a}^{b}|f-g| |g-h|\,d\alpha \right| \\
		&\leq \left\{ \int_{a}^{b} |f-g|^2\,d\alpha \right\}^{\frac{1}{2}} \left\{ \int_{a}^{b} |g-h|^2\,d\alpha \right\}^{\frac{1}{2}} \\
		&= \| f-g \|_2~\|g-h\|_2.
		\end{align*}
		So,
		\begin{align*}
		\|f-h\|^2_2
		&= \int_{a}^{b} |f-h|^2\,d\alpha \\
		&= \int_{a}^{b} |(f-g)+(g-h)|^2\,d\alpha \\
		&= \int_{a}^{b} |(f-g)|^2\,d\alpha + 2\int_{a}^{b} |(f-g)| |(g-h)|\,d\alpha+ \int_{a}^{b}|(g-h)|^2\,d\alpha \\
		&\leq \|f-g\|^2_2 + 2~\|f-g\|_2~\|g-h\|_2 + \|g-h\|^2_2 \\
		&= (\|f-g\|_2 + \|g-h\|_2)^2.
		\end{align*}
		It follows that
		$$
		\|f-h\|_2 \leq \|f-g\|_2 + \|g-h\|_2.
		$$
	\end{proof}
\end{Exercise}