% === Exercise 5.6 ===
\begin{Exercise}
	\begin{proof}
		It suffice to prove $g'(x) \geq 0$ for all $x>0$.
		Since $f$ is continuous on $[0,\infty)$ and $f$ is differentiable on $(0,\infty)$, by the Mean Value Theorem, we have
		$$
		f(x) - f(0) = f'(c)(x-0)
		$$
		where $c\in(0,x)$.
		Using the hypothesis that $f(0) = 0$, we obtain
		$$
		f'(c) = \frac{f(x)}{x}.
		$$
		Since $f'$ is monotonically increasing, we know
		$$
		x\geq c \implies f'(x) \geq f'(c).
		$$
		It follows that
		$$
		g'(x) 
		= \frac{xf'(x) - f(x)}{x^2} 
		\geq \frac{xf'(c) - f(x)}{x^2}
		= \frac{x \cdot \frac{f(x)}{x} - f(x)}{x^2}
		= 0
		$$
		for all $x>0$.
		Hence $g$ is monotonically increasing.
	\end{proof}
\end{Exercise}