% === Exercise 5.22 ===
\begin{Exercise}
\begin{enumerate}[(a)]
\item 
\begin{proof}
Suppose to contrary that $f$ has more than one fixed point, says $x_1$, $x_2$.
Notice that $x_1\neq x_2$.
Then by Mean Value Theorem, we consider
$$
f'(t) = \frac{f(x_1)-f(x_2)}{x_1-x_2}
= \frac{x_1-x_2}{x_1-x_2}
=1
$$
where $t\in (x_1,x_2)$.
This contradicts $f'(t) \neq 1$ for all $t$.
Hence $f$ has at most one fixed point.
\end{proof}

\item
\begin{proof}
We observe
$$
f'(t) = 1-\frac{e^t}{(1+e^t)^2}.
$$
This means $0<f'(t)<1$ for all $t$.
Suppose to contrary there exists a fixed point $t_0\in\mathbb{R}$ such that $f(t_0) = t_0$.
Then $f(t_0) = t_0 + (1+e^t_0)^{-1}$ implies $e^{t_0} = 0$.
There is no $t_0\in\mathbb{R}$ satisfied so is a contradiction.
It follows that $f$ has no fixed point.
\end{proof}

\item
\begin{proof}
Since $|f'(t)| \leq A$ for all $t$, then
$$
\left| \frac{f(x_{n+1})-f(x_n)}{x_{n+1}-x_n} \right | \leq A
$$
which implies
$$
\left| f(x_{n+1})-f(x_n) \right| \leq A \left| x_{n+1}-x_n \right|.
$$
This inequality holds for all $n\in\mathbb{N}$. By induction, we have
$$
|f(x_{n+1})-f(x_n)| \leq A^n | x_2-x_1 |.
$$
Notice that $A < 1$, for $k > 0$, we consider
\begin{align*}
| x_{n+k} - x_n |
&\leq |x_{n+k}-x_{n+k-1}| + |x_{n+k-1}-x_{n+k-2}| + \cdots + | x_2 - x_1 | \\
&= A^{n+k-2} |x_2-x_1| + A^{n+k-3} |x_2-x_1| + \cdots + A^{n-1} |x_2 - x_1| \\
&\leq k A^{n-1} | x_2-x_1 |.
\end{align*}
Taking the limit on both sides as $n\to\infty$, we have
$$
\lim_{n\to\infty} |x_{n+k}-x_n| \leq 0.
$$
Hence $\lim_{n\to\infty}|x_{n+k}-x_n| = 0$, it follows that the sequence $\{x_k\}$ is Cauchy.
Since $\mathbb{R}$ is compact, then by Theorem 3.11(b), we know there is $x\in\mathbb{R}$ such that 
$$
\lim_{n\to\infty} x_n = x.
$$
Moreover, by definition of $f(x_n)$, we also have 
$$
\lim_{n\to\infty} f(x_n) = x.
$$
Since $f'(t)$ exists for all $t\in\mathbb{R}$ by hypothesis, then $f$ is continuous on $\mathbb{R}$, we conclude
$$
f(x) = x
$$
which means $x$ is a fixed point of $f$.
\end{proof}

\item
\begin{solution}
Consider the points $\big(x_n, f(x_n)\big)$.
We know when $n\to\infty$, the point must be a fixed point $(x, x)$.
If we start with $\big(x_1, f(x_1)\big)$, then we want to arrive at $\big(x_2, f(x_2)\big)$. We just pick the path
$$
\big(x_1, f(x_1)\big) \to \big(x_2, f(x_1)\big) \to \big(x_2, f(x_2)\big)
$$
which means
$$
\big(x_1, x_2\big) \to \big(x_2, x_2\big) \to \big(x_2, x_3\big).
$$
Then we arrive at $\big(x_3, f(x_3)\big)$, which means

$$
\big(x_2, x_3\big) \to \big(x_3, x_3\big) \to \big(x_3, x_4\big).
$$
This process continue until we arrive at the fixed point.
By induction, we obtain the zig-zag path.
\end{solution}
\end{enumerate}
\end{Exercise}