% === Exercise 5.17 ===
\begin{Exercise}
	\begin{proof}
		Follow the hint.
		By Theorem 5.15 (Taylor's Theorem), if we put $\alpha = 0, \beta = 1$, then
		$$
		f(1) = f(0) + f'(0) + \frac{f''(0)}{2}+\frac{f^{(3)}(s)}{6}
		$$
		where $s\in(0,1)$.
		If we put $\alpha = 0, \beta = -1$, then
		$$
		f(-1) = f(0) - f'(0) + \frac{f''(0)}{2}-\frac{f^{(3)}(t)}{6}
		$$
		where $t\in(-1,0)$.
		Now we subtract the second equation from the first one so that
		$$
		f(1) + f(-1) = 2f'(0) + \frac{f^{(3)}(s)}{6} + \frac{f^{(3)}(t)}{6}.
		$$
		Since $f(1) = 1, f(-1) = 0, f'(0) = 0$, we have
		$$
		\frac{f^{(3)}(s)}{6} + \frac{f^{(3)}(t)}{6} = 1
		$$
		where $s\in(0,1), t\in(-1,0)$.
		We deduce
		$$
		f^{(3)}(s) + f^{(3)}(t) = 6
		$$
		where $s,t\in(-1,1)$.
		This is the desired result to conclude
		$$
		f^{(3)}(x) \geq 3
		$$
		for some $x\in(-1,1)$.
	\end{proof}
\end{Exercise}